<?xml version="1.0" encoding="UTF-8"?>
<rdf:RDF xmlns="http://data.europa.eu/a4g/ontology#"
         xmlns:adms="http://www.w3.org/ns/adms#"
         xmlns:at="http://publications.europa.eu/ontology/authority/"
         xmlns:at-voc="http://publications.europa.eu/resource/authority/"
         xmlns:at-voc-new="http://publications.europa.eu/resource/authority/new/"
         xmlns:atold="http://publications.europa.eu/resource/authority/"
         xmlns:cccev="http://data.europa.eu/m8g/"
         xmlns:core="http://data.europa.eu/m8g/"
         xmlns:cpov="http://data.europa.eu/m8g/"
         xmlns:cpsv="http://data.europa.eu/m8g/"
         xmlns:cpv="http://data.europa.eu/m8g/"
         xmlns:cv="http://data.europa.eu/m8g/"
         xmlns:dc="http://purl.org/dc/elements/1.1/"
         xmlns:dct="http://purl.org/dc/terms/"
         xmlns:dul="http://www.ontologydesignpatterns.org/ont/dul/DUL.owl#"
         xmlns:espd="https://github.com/ESPD/ESPD-EDM/"
         xmlns:euvoc="http://publications.europa.eu/ontology/euvoc#"
         xmlns:foaf="http://xmlns.com/foaf/0.1/"
         xmlns:geosparql="http://www.opengis.net/ont/geosparql#"
         xmlns:lexinfo="http://www.lexinfo.net/ontology/2.0/lexinfo#"
         xmlns:lexvo="http://lexvo.org/ontology#"
         xmlns:locn="http://www.w3.org/ns/locn#"
         xmlns:nuts="http://data.europa.eu/nuts/"
         xmlns:org="http://www.w3.org/ns/org#"
         xmlns:owl="http://www.w3.org/2002/07/owl#"
         xmlns:person="http://www.w3.org/ns/person#"
         xmlns:rdf="http://www.w3.org/1999/02/22-rdf-syntax-ns#"
         xmlns:rdfs="http://www.w3.org/2000/01/rdf-schema#"
         xmlns:sf="http://www.opengis.net/ont/sf#"
         xmlns:skos="http://www.w3.org/2004/02/skos/core#"
         xmlns:skosxl="http://www.w3.org/2008/05/skos-xl#"
         xmlns:time="http://www.w3.org/2006/time#"
         xmlns:vann="http://purl.org/vocab/vann/"
         xmlns:vcard="http://www.w3.org/2006/vcard/ns#"
         xmlns:wgs="http://www.w3.org/2003/01/geo/wgs84_pos#"
         xmlns:xsd="http://www.w3.org/2001/XMLSchema#">
   <owl:Ontology rdf:about="http://data.europa.eu/a4g/ontology#curr">
      <owl:imports rdf:resource="http://xmlns.com/foaf/0.1/"/>
      <owl:imports rdf:resource="http://purl.org/dc/terms/"/>
      <owl:imports rdf:resource="http://www.w3.org/ns/org#"/>
      <owl:imports rdf:resource="http://www.w3.org/2004/02/skos/core"/>
      <owl:imports rdf:resource="http://data.europa.eu/nuts"/>
      <owl:imports rdf:resource="ttp://publications.europa.eu/ontology/authority/"/>
      <owl:imports rdf:resource="http://publications.europa.eu/resource/authority/"/>
      <owl:imports rdf:resource="http://www.w3.org/2006/time"/>
      <owl:imports rdf:resource="http://www.w3.org/ns/locn"/>
      <owl:imports rdf:resource="https://data.europa.eu/m8g/"/>
      <owl:imports rdf:resource="http://data.europa.eu/m8g/"/>
      <owl:imports rdf:resource="http://data.europa.eu/m8g/"/>
      <owl:imports rdf:resource="http://data.europa.eu/m8g/"/>
      <owl:imports rdf:resource="http://data.europa.eu/m8g/"/>
      <owl:imports rdf:resource="https://data.europa.eu/m8g/"/>
      <owl:imports rdf:resource="http://www.opengis.net/ont/geosparql"/>
      <owl:imports rdf:resource="http://www.w3.org/ns/person"/>
      <owl:imports rdf:resource="http://www.w3.org/ns/adms"/>
      <owl:imports rdf:resource="http://www.w3.org/2003/01/geo/wgs84_pos"/>
      <owl:imports rdf:resource="http://publications.europa.eu/ontology/euvoc"/>
      <owl:imports rdf:resource="http://lexvo.org/ontology"/>
      <owl:imports rdf:resource="http://www.w3.org/2008/05/skos-xl"/>
      <owl:imports rdf:resource="http://www.lexinfo.net/ontology/2.0/lexinfo"/>
      <owl:imports rdf:resource="http://www.w3.org/2006/vcard/ns"/>
      <owl:imports rdf:resource="http://publications.europa.eu/resource/authority/"/>
      <owl:imports rdf:resource="http://www.opengis.net/ont/sf"/>
      <dct:title xml:lang="en">eProcurement Ontology Catalogue - core</dct:title>
      <rdfs:label xml:lang="en">Core Public Organisation Vocabulary - core</rdfs:label>
      <dct:description xml:lang="en">The eProcurement Ontology Catalogue core describes the concepts and properties representing the European Public Procurement Catalogue domain. The provision of these semantics offers the basis for a common understanding of the domain for all stakeholders ensuring the quality of data exchange and transparency. The ontology restrictions are published in a separate artefact.</dct:description>
      <dct:publisher>http://publications.europa.eu/resource/authority/corporate-body/PUBL</dct:publisher>
      <rdfs:comment>This version is automatically generated from currency_src_ap_CM.xml on 2024-02-13</rdfs:comment>
      <rdfs:seeAlso rdf:resource="https://github.com/OP-TED/ePO/releases"/>
      <rdfs:seeAlso rdf:resource="https://joinup.ec.europa.eu/collection/eprocurement/solution/eprocurement-ontology/about"/>
      <rdfs:seeAlso rdf:resource="https://op.europa.eu/en/web/eu-vocabularies/e-procurement"/>
      <rdfs:seeAlso rdf:resource="https://docs.ted.europa.eu/home/index.html"/>
      <dct:issued rdf:datatype="http://www.w3.org/2001/XMLSchema#date">2024-02-13</dct:issued>
      <dct:created rdf:datatype="http://www.w3.org/2001/XMLSchema#date">2021-06-01</dct:created>
      <owl:versionInfo>4.1.1</owl:versionInfo>
      <owl:incompatibleWith>3.1.2</owl:incompatibleWith>
      <owl:versionIRI rdf:resource="http://data.europa.eu/a4g/ontology#curr-4.1.1"/>
      <owl:priorVersion>http://data.europa.eu/a4g/ontology#curr-3.1.2</owl:priorVersion>
      <vann:preferredNamespaceUri>http://data.europa.eu/a4g/ontology#</vann:preferredNamespaceUri>
      <vann:preferredNamespacePrefix>epo</vann:preferredNamespacePrefix>
      <dct:license>© European Union, 2014. Unless otherwise noted, the reuse of the Ontology is authorised under the European Union Public Licence v1.2 (https://eupl.eu/).</dct:license>
   </owl:Ontology>
   <owl:Class rdf:about="http://publications.europa.eu/ontology/euvoc#Currency"/>
   <rdf:Description rdf:about="http://publications.europa.eu/ontology/euvoc#Currency">
      <skos:prefLabel xml:lang="en">Currency</skos:prefLabel>
   </rdf:Description>
   <skos:ConceptScheme rdf:about="http://publications.europa.eu/resource/authority/currency"/>
   <rdf:Description rdf:about="http://publications.europa.eu/resource/authority/currency">
      <skos:prefLabel xml:lang="en">Currency</skos:prefLabel>
   </rdf:Description>
   <rdf:Description rdf:about="http://publications.europa.eu/resource/authority/currency">
      <skos:definition xml:lang="en">The Currency authority table is a controlled vocabulary that lists concepts associated with currencies and currency subunits. The concepts included are correlated with the ISO 4217 international standard. The Currency authority table is updated based on the stakeholders’ needs.</skos:definition>
   </rdf:Description>
   <owl:Class rdf:about="http://publications.europa.eu/ontology/euvoc#Currency">
      <rdfs:subClassOf rdf:resource="http://www.w3.org/2004/02/skos/core#Concept"/>
   </owl:Class>
   <owl:ObjectProperty rdf:about="http://publications.europa.eu/ontology/euvoc#usedIn"/>
   <rdf:Description rdf:about="http://publications.europa.eu/ontology/euvoc#usedIn">
      <skos:prefLabel xml:lang="en">Used in</skos:prefLabel>
   </rdf:Description>
   <rdf:Description rdf:about="http://publications.europa.eu/ontology/euvoc#usedIn">
      <skos:definition xml:lang="en">It indicates that the currency is used in or associated with the specified country. (euvoc:Currency -&gt; at-voc:country (+euvoc:usedIn))</skos:definition>
   </rdf:Description>
   <owl:ObjectProperty rdf:about="http://www.w3.org/2004/02/skos/core#inScheme"/>
   <rdf:Description rdf:about="http://www.w3.org/2004/02/skos/core#inScheme">
      <skos:prefLabel xml:lang="en">In scheme</skos:prefLabel>
   </rdf:Description>
   <rdf:Description rdf:about="http://www.w3.org/2004/02/skos/core#inScheme">
      <skos:definition xml:lang="en">A concept scheme in which the concept is included. A concept may be a member of more than one concept scheme. (euvoc:Currency -&gt; at-voc:currency (+skos:inScheme))</skos:definition>
   </rdf:Description>
   <owl:DatatypeProperty rdf:about="http://publications.europa.eu/ontology/euvoc#decimalPlace"/>
   <rdf:Description rdf:about="http://publications.europa.eu/ontology/euvoc#decimalPlace">
      <skos:prefLabel xml:lang="en">Decimal place</skos:prefLabel>
   </rdf:Description>
</rdf:RDF>
