@prefix : <http://data.europa.eu/a4g/ontology#> .
@prefix at-voc: <http://publications.europa.eu/resource/authority/> .
@prefix cccev: <http://data.europa.eu/m8g/> .
@prefix dcterms: <http://purl.org/dc/terms/> .
@prefix euvoc: <http://publications.europa.eu/ontology/euvoc#> .
@prefix foaf: <http://xmlns.com/foaf/0.1/> .
@prefix org: <http://www.w3.org/ns/org#> .
@prefix owl: <http://www.w3.org/2002/07/owl#> .
@prefix rdfs: <http://www.w3.org/2000/01/rdf-schema#> .
@prefix skos: <http://www.w3.org/2004/02/skos/core#> .
@prefix vann: <http://purl.org/vocab/vann/> .
@prefix xsd: <http://www.w3.org/2001/XMLSchema#> .

:curr a owl:Ontology ;
    rdfs:label "Core Public Organisation Vocabulary - core"@en ;
    dcterms:created "2021-06-01"^^xsd:date ;
    dcterms:description "The eProcurement Ontology Catalogue core describes the concepts and properties representing the European Public Procurement Catalogue domain. The provision of these semantics offers the basis for a common understanding of the domain for all stakeholders ensuring the quality of data exchange and transparency. The ontology restrictions are published in a separate artefact."@en ;
    dcterms:issued "2024-03-08"^^xsd:date ;
    dcterms:license "© European Union, 2014. Unless otherwise noted, the reuse of the Ontology is authorised under the European Union Public Licence v1.2 (https://eupl.eu/)." ;
    dcterms:publisher "http://publications.europa.eu/resource/authority/corporate-body/PUBL" ;
    dcterms:title "eProcurement Ontology Catalogue - core"@en ;
    vann:preferredNamespacePrefix "epo" ;
    vann:preferredNamespaceUri "http://data.europa.eu/a4g/ontology#" ;
    rdfs:comment "This version is automatically generated from currency_src_ap_CM.xml on 2024-03-08" ;
    rdfs:seeAlso <https://docs.ted.europa.eu/home/index.html>,
        <https://github.com/OP-TED/ePO/releases>,
        <https://joinup.ec.europa.eu/collection/eprocurement/solution/eprocurement-ontology/about>,
        <https://op.europa.eu/en/web/eu-vocabularies/e-procurement> ;
    owl:imports cccev:,
        <http://data.europa.eu/nuts>,
        <http://lexvo.org/ontology>,
        <http://publications.europa.eu/ontology/euvoc>,
        at-voc:,
        dcterms:,
        <http://www.lexinfo.net/ontology/2.0/lexinfo>,
        <http://www.opengis.net/ont/geosparql>,
        <http://www.opengis.net/ont/sf>,
        <http://www.w3.org/2003/01/geo/wgs84_pos>,
        <http://www.w3.org/2004/02/skos/core>,
        <http://www.w3.org/2006/time>,
        <http://www.w3.org/2006/vcard/ns>,
        <http://www.w3.org/2008/05/skos-xl>,
        <http://www.w3.org/ns/adms>,
        <http://www.w3.org/ns/locn>,
        org:,
        <http://www.w3.org/ns/person>,
        foaf:,
        <https://data.europa.eu/m8g/>,
        <ttp://publications.europa.eu/ontology/authority/> ;
    owl:incompatibleWith "3.1.2" ;
    owl:priorVersion "http://data.europa.eu/a4g/ontology#curr-3.1.2" ;
    owl:versionIRI :curr-4.1.1 ;
    owl:versionInfo "4.1.1" .

euvoc:Currency a owl:Class ;
    rdfs:subClassOf skos:Concept ;
    skos:prefLabel "Currency"@en .

euvoc:decimalPlace a owl:DatatypeProperty ;
    skos:prefLabel "Decimal place"@en .

euvoc:usedIn a owl:ObjectProperty ;
    skos:definition "It indicates that the currency is used in or associated with the specified country. (euvoc:Currency -> at-voc:country (+euvoc:usedIn))"@en ;
    skos:prefLabel "Used in"@en .

at-voc:currency a skos:ConceptScheme ;
    skos:definition "The Currency authority table is a controlled vocabulary that lists concepts associated with currencies and currency subunits. The concepts included are correlated with the ISO 4217 international standard. The Currency authority table is updated based on the stakeholders’ needs."@en ;
    skos:prefLabel "Currency"@en .

skos:inScheme a owl:ObjectProperty ;
    skos:definition "A concept scheme in which the concept is included. A concept may be a member of more than one concept scheme. (euvoc:Currency -> at-voc:currency (+skos:inScheme))"@en ;
    skos:prefLabel "In scheme"@en .

