@prefix : <http://data.europa.eu/a4g/ontology#> .
@prefix at-voc: <http://publications.europa.eu/resource/authority/> .
@prefix cccev: <http://data.europa.eu/m8g/> .
@prefix dcterms: <http://purl.org/dc/terms/> .
@prefix euvoc: <http://publications.europa.eu/ontology/euvoc#> .
@prefix foaf: <http://xmlns.com/foaf/0.1/> .
@prefix org: <http://www.w3.org/ns/org#> .
@prefix owl: <http://www.w3.org/2002/07/owl#> .
@prefix rdfs: <http://www.w3.org/2000/01/rdf-schema#> .
@prefix skos: <http://www.w3.org/2004/02/skos/core#> .
@prefix vann: <http://purl.org/vocab/vann/> .
@prefix wgs1: <http://www.w3.org/2003/01/geo/wgs84_pos#> .
@prefix xsd: <http://www.w3.org/2001/XMLSchema#> .

:cob a owl:Ontology ;
    rdfs:label "Core Public Organisation Vocabulary - core"@en ;
    dcterms:created "2021-06-01"^^xsd:date ;
    dcterms:description "The eProcurement Ontology Catalogue core describes the concepts and properties representing the European Public Procurement Catalogue domain. The provision of these semantics offers the basis for a common understanding of the domain for all stakeholders ensuring the quality of data exchange and transparency. The ontology restrictions are published in a separate artefact."@en ;
    dcterms:issued "2023-12-01"^^xsd:date ;
    dcterms:license "© European Union, 2014. Unless otherwise noted, the reuse of the Ontology is authorised under the European Union Public Licence v1.2 (https://eupl.eu/)." ;
    dcterms:publisher "http://publications.europa.eu/resource/authority/corporate-body/PUBL" ;
    dcterms:title "eProcurement Ontology Catalogue - core"@en ;
    vann:preferredNamespacePrefix "epo" ;
    vann:preferredNamespaceUri "http://data.europa.eu/a4g/ontology#" ;
    rdfs:comment "This version is automatically generated from cob_src_ap_CM.xml on 2023-12-01" ;
    rdfs:seeAlso <https://docs.ted.europa.eu/home/index.html>,
        <https://github.com/OP-TED/ePO/releases>,
        <https://joinup.ec.europa.eu/collection/eprocurement/solution/eprocurement-ontology/about>,
        <https://op.europa.eu/en/web/eu-vocabularies/e-procurement> ;
    owl:imports cccev:,
        <http://data.europa.eu/nuts>,
        <http://lexvo.org/ontology>,
        <http://publications.europa.eu/ontology/euvoc>,
        at-voc:,
        dcterms:,
        <http://www.lexinfo.net/ontology/2.0/lexinfo>,
        <http://www.opengis.net/ont/geosparql>,
        <http://www.opengis.net/ont/sf>,
        <http://www.w3.org/2003/01/geo/wgs84_pos>,
        <http://www.w3.org/2004/02/skos/core>,
        <http://www.w3.org/2006/time>,
        <http://www.w3.org/2006/vcard/ns>,
        <http://www.w3.org/2008/05/skos-xl>,
        <http://www.w3.org/ns/adms>,
        <http://www.w3.org/ns/locn>,
        org:,
        <http://www.w3.org/ns/person>,
        foaf:,
        <https://data.europa.eu/m8g/>,
        <ttp://publications.europa.eu/ontology/authority/> ;
    owl:incompatibleWith "3.1.1" ;
    owl:priorVersion "http://data.europa.eu/a4g/ontology#cob-3.1.1" ;
    owl:versionIRI :cob-4.1.0 ;
    owl:versionInfo "4.1.0" .

euvoc:CorporateBody a owl:Class ;
    rdfs:subClassOf skos:Concept ;
    skos:definition "A conceptual entity represents the abstract notion of corporate bodies. This concept serves as a controlled vocabulary, offering varying names of European Union (EU) corporate bodies."@en ;
    skos:prefLabel "Corporate body"@en .

euvoc:hasPrimaryContactPoint a owl:ObjectProperty ;
    skos:definition "It indicate the primary means of contact for an entity (e.g., an organization or corporate body), linking that entity to a specific contact point (euvoc:CorporateBody -> vcard:ContactPoint (+euvoc:hasPrimaryContactPoint))"@en ;
    skos:prefLabel "Has primary contact point"@en .

euvoc:legallyBasedOnTreaty a owl:ObjectProperty ;
    skos:definition "It indicates that the corporate body's operations, existence, or functions are legally grounded in or regulated by the terms and provisions of the specified treaty. (euvoc:CorporateBody -> euvoc:Treaty (+euvoc:legallyBasedOnTreaty))"@en ;
    skos:prefLabel "Legally based on treaty"@en .

euvoc:managedBy a owl:ObjectProperty ;
    skos:prefLabel "Managed by"@en .

euvoc:order a owl:DatatypeProperty ;
    skos:prefLabel "Order"@en .

at-voc:corporate-body a owl:NamedIndividual,
        skos:ConceptScheme ;
    skos:definition "The Corporate body authority table is a controlled vocabulary which provides the varying names of EU corporate bodies for a given time span. Some other – international and national – corporate bodies are also included as far as they are used in the various systems in the Publications Office. The traceability of the chronological modifications is ensured when possible."@en ;
    skos:prefLabel "Corporate-body"@en .

wgs1:location a owl:ObjectProperty ;
    skos:definition "It is used to precisely indicate a location's position. (euvoc:CorporateBody -> euvoc:Place (+wgs:location))"@en ;
    skos:prefLabel "Location"@en .

skos:inScheme a owl:ObjectProperty ;
    skos:definition "A concept scheme in which the concept is included. A concept may be a member of more than one concept scheme. (euvoc:CorporateBody -> at-voc:corporate-body (+skos:inScheme))"@en ;
    skos:prefLabel "In scheme"@en .

org:siteOf a owl:ObjectProperty ;
    skos:prefLabel "Site of"@en .

foaf:homepage a owl:DatatypeProperty ;
    skos:definition "The main web page used by the instance of the concept. (euvoc:CorporateBody)"@en ;
    skos:prefLabel "Homepage"@en .

