<?xml version="1.0" encoding="UTF-8"?>
<rdf:RDF xmlns="http://data.europa.eu/a4g/ontology#"
         xmlns:adms="http://www.w3.org/ns/adms#"
         xmlns:at="http://publications.europa.eu/ontology/authority/"
         xmlns:at-voc="http://publications.europa.eu/resource/authority/"
         xmlns:at-voc-new="http://publications.europa.eu/resource/authority/new/"
         xmlns:atold="http://publications.europa.eu/resource/authority/"
         xmlns:cccev="http://data.europa.eu/m8g/"
         xmlns:core="http://data.europa.eu/m8g/"
         xmlns:cpov="http://data.europa.eu/m8g/"
         xmlns:cpsv="http://data.europa.eu/m8g/"
         xmlns:cpv="http://data.europa.eu/m8g/"
         xmlns:cv="http://data.europa.eu/m8g/"
         xmlns:dc="http://purl.org/dc/elements/1.1/"
         xmlns:dct="http://purl.org/dc/terms/"
         xmlns:dul="http://www.ontologydesignpatterns.org/ont/dul/DUL.owl#"
         xmlns:espd="https://github.com/ESPD/ESPD-EDM/"
         xmlns:euvoc="http://publications.europa.eu/ontology/euvoc#"
         xmlns:foaf="http://xmlns.com/foaf/0.1/"
         xmlns:geosparql="http://www.opengis.net/ont/geosparql#"
         xmlns:lexinfo="http://www.lexinfo.net/ontology/2.0/lexinfo#"
         xmlns:lexvo="http://lexvo.org/ontology#"
         xmlns:locn="http://www.w3.org/ns/locn#"
         xmlns:nuts="http://data.europa.eu/nuts/"
         xmlns:org="http://www.w3.org/ns/org#"
         xmlns:owl="http://www.w3.org/2002/07/owl#"
         xmlns:person="http://www.w3.org/ns/person#"
         xmlns:rdf="http://www.w3.org/1999/02/22-rdf-syntax-ns#"
         xmlns:rdfs="http://www.w3.org/2000/01/rdf-schema#"
         xmlns:sf="http://www.opengis.net/ont/sf#"
         xmlns:skos="http://www.w3.org/2004/02/skos/core#"
         xmlns:skosxl="http://www.w3.org/2008/05/skos-xl#"
         xmlns:time="http://www.w3.org/2006/time#"
         xmlns:vann="http://purl.org/vocab/vann/"
         xmlns:vcard="http://www.w3.org/2006/vcard/ns#"
         xmlns:wgs="http://www.w3.org/2003/01/geo/wgs84_pos#"
         xmlns:xsd="http://www.w3.org/2001/XMLSchema#">
   <owl:Ontology rdf:about="http://data.europa.eu/a4g/ontology#tech">
      <owl:imports rdf:resource="http://xmlns.com/foaf/0.1/"/>
      <owl:imports rdf:resource="http://purl.org/dc/terms/"/>
      <owl:imports rdf:resource="http://www.w3.org/ns/org#"/>
      <owl:imports rdf:resource="http://www.w3.org/2004/02/skos/core"/>
      <owl:imports rdf:resource="http://data.europa.eu/nuts"/>
      <owl:imports rdf:resource="ttp://publications.europa.eu/ontology/authority/"/>
      <owl:imports rdf:resource="http://publications.europa.eu/resource/authority/"/>
      <owl:imports rdf:resource="http://www.w3.org/2006/time"/>
      <owl:imports rdf:resource="http://www.w3.org/ns/locn"/>
      <owl:imports rdf:resource="https://data.europa.eu/m8g/"/>
      <owl:imports rdf:resource="http://data.europa.eu/m8g/"/>
      <owl:imports rdf:resource="http://data.europa.eu/m8g/"/>
      <owl:imports rdf:resource="http://data.europa.eu/m8g/"/>
      <owl:imports rdf:resource="http://data.europa.eu/m8g/"/>
      <owl:imports rdf:resource="https://data.europa.eu/m8g/"/>
      <owl:imports rdf:resource="http://www.opengis.net/ont/geosparql"/>
      <owl:imports rdf:resource="http://www.w3.org/ns/person"/>
      <owl:imports rdf:resource="http://www.w3.org/ns/adms"/>
      <owl:imports rdf:resource="http://www.w3.org/2003/01/geo/wgs84_pos"/>
      <owl:imports rdf:resource="http://publications.europa.eu/ontology/euvoc"/>
      <owl:imports rdf:resource="http://lexvo.org/ontology"/>
      <owl:imports rdf:resource="http://www.w3.org/2008/05/skos-xl"/>
      <owl:imports rdf:resource="http://www.lexinfo.net/ontology/2.0/lexinfo"/>
      <owl:imports rdf:resource="http://www.w3.org/2006/vcard/ns"/>
      <owl:imports rdf:resource="http://publications.europa.eu/resource/authority/"/>
      <owl:imports rdf:resource="http://www.opengis.net/ont/sf"/>
      <dct:title xml:lang="en">technical package  - core</dct:title>
      <rdfs:label xml:lang="en">Core Public Organisation Vocabulary - core</rdfs:label>
      <dct:description xml:lang="en">The common SRC_AP Ontology core describes the concepts and properties representing the European Public Procurement Catalogue domain. The provision of these semantics offers the basis for a common understanding of the domain for all stakeholders ensuring the quality of data exchange and transparency. The ontology restrictions are published in a separate artefact.</dct:description>
      <dct:publisher>http://publications.europa.eu/resource/authority/corporate-body/PUBL</dct:publisher>
      <rdfs:comment>This version is automatically generated from common_src_ap_CM.xml on 2024-02-27</rdfs:comment>
      <rdfs:seeAlso rdf:resource="https://github.com/OP-TED/ePO/releases"/>
      <rdfs:seeAlso rdf:resource="https://joinup.ec.europa.eu/collection/eprocurement/solution/eprocurement-ontology/about"/>
      <rdfs:seeAlso rdf:resource="https://op.europa.eu/en/web/eu-vocabularies/e-procurement"/>
      <rdfs:seeAlso rdf:resource="https://docs.ted.europa.eu/home/index.html"/>
      <dct:issued rdf:datatype="http://www.w3.org/2001/XMLSchema#date">2024-02-27</dct:issued>
      <dct:created rdf:datatype="http://www.w3.org/2001/XMLSchema#date">2021-06-01</dct:created>
      <owl:versionInfo>4.0.0</owl:versionInfo>
      <owl:incompatibleWith>3.1.0</owl:incompatibleWith>
      <owl:versionIRI rdf:resource="http://data.europa.eu/a4g/ontology#tech-4.0.0"/>
      <owl:priorVersion>http://data.europa.eu/a4g/ontology#tech-3.1.0</owl:priorVersion>
      <vann:preferredNamespaceUri>http://data.europa.eu/a4g/ontology#</vann:preferredNamespaceUri>
      <vann:preferredNamespacePrefix>epo</vann:preferredNamespacePrefix>
      <dct:license>Â© European Union, 2014. Unless otherwise noted, the reuse of the Ontology is authorised under the European Union Public Licence v1.2 (https://eupl.eu/).</dct:license>
   </owl:Ontology>
   <owl:Class rdf:about="http://publications.europa.eu/ontology/euvoc#ConceptStatus"/>
   <rdf:Description rdf:about="http://publications.europa.eu/ontology/euvoc#ConceptStatus">
      <skos:prefLabel xml:lang="en">Concept status</skos:prefLabel>
   </rdf:Description>
   <rdf:Description rdf:about="http://publications.europa.eu/ontology/euvoc#ConceptStatus">
      <skos:definition xml:lang="en">It categorizes or represents concept statuses within the EU Vocabularies.</skos:definition>
   </rdf:Description>
   <owl:Class rdf:about="http://publications.europa.eu/ontology/euvoc#CorrectionStatus"/>
   <rdf:Description rdf:about="http://publications.europa.eu/ontology/euvoc#CorrectionStatus">
      <skos:prefLabel xml:lang="en">Correction status</skos:prefLabel>
   </rdf:Description>
   <rdf:Description rdf:about="http://publications.europa.eu/ontology/euvoc#CorrectionStatus">
      <skos:definition xml:lang="en">The Correction status authority table (AT) provides the possible statuses of proofreading of labels and descriptions.</skos:definition>
   </rdf:Description>
   <owl:Class rdf:about="http://publications.europa.eu/ontology/euvoc#GrammaticalGender"/>
   <rdf:Description rdf:about="http://publications.europa.eu/ontology/euvoc#GrammaticalGender">
      <skos:prefLabel xml:lang="en">Grammatical gender</skos:prefLabel>
   </rdf:Description>
   <owl:Class rdf:about="http://publications.europa.eu/ontology/euvoc#GrammaticalNumber"/>
   <rdf:Description rdf:about="http://publications.europa.eu/ontology/euvoc#GrammaticalNumber">
      <skos:prefLabel xml:lang="en">Grammatical number</skos:prefLabel>
   </rdf:Description>
   <owl:Class rdf:about="http://publications.europa.eu/ontology/euvoc#LabelType"/>
   <rdf:Description rdf:about="http://publications.europa.eu/ontology/euvoc#LabelType">
      <skos:prefLabel xml:lang="en">Label type</skos:prefLabel>
   </rdf:Description>
   <rdf:Description rdf:about="http://publications.europa.eu/ontology/euvoc#LabelType">
      <skos:definition xml:lang="en">The label-type authority table is a controlled vocabulary providing the various forms of labels that are considered alternative labels in the SKOS format. This authority table is an internal table at the Publications Office of the European Union.</skos:definition>
   </rdf:Description>
   <owl:Class rdf:about="http://publications.europa.eu/ontology/euvoc#NotationType"/>
   <rdf:Description rdf:about="http://publications.europa.eu/ontology/euvoc#NotationType">
      <skos:prefLabel xml:lang="en">Notation type</skos:prefLabel>
   </rdf:Description>
   <rdf:Description rdf:about="http://publications.europa.eu/ontology/euvoc#NotationType">
      <skos:definition xml:lang="en">A conceptual entity represents the notation types within the EU Vocabularies.</skos:definition>
   </rdf:Description>
   <owl:Class rdf:about="http://publications.europa.eu/ontology/euvoc#Script"/>
   <rdf:Description rdf:about="http://publications.europa.eu/ontology/euvoc#Script">
      <skos:prefLabel xml:lang="en">Script</skos:prefLabel>
   </rdf:Description>
   <owl:Class rdf:about="http://publications.europa.eu/ontology/euvoc#UseContext"/>
   <rdf:Description rdf:about="http://publications.europa.eu/ontology/euvoc#UseContext">
      <skos:prefLabel xml:lang="en">Use context</skos:prefLabel>
   </rdf:Description>
   <rdf:Description rdf:about="http://publications.europa.eu/ontology/euvoc#UseContext">
      <skos:definition xml:lang="en">Provides different applications and environments that make use of the various controlled vocabularies.</skos:definition>
   </rdf:Description>
   <owl:Class rdf:about="http://publications.europa.eu/ontology/euvoc#XlNotation"/>
   <rdf:Description rdf:about="http://publications.europa.eu/ontology/euvoc#XlNotation">
      <skos:prefLabel xml:lang="en">Xl notation</skos:prefLabel>
   </rdf:Description>
   <rdf:Description rdf:about="http://publications.europa.eu/ontology/euvoc#XlNotation">
      <skos:definition xml:lang="en">A notation is a string of characters used to uniquely identify a concept within a specified context. Like the skosxl:Label class reifies SKOS label statements, XlNotation reifies SKOS notation statements. This class permits, if needed, to maintain the historical view of the values and add additional provenance descriptions.</skos:definition>
   </rdf:Description>
   <owl:Class rdf:about="http://publications.europa.eu/ontology/euvoc#XlNote"/>
   <rdf:Description rdf:about="http://publications.europa.eu/ontology/euvoc#XlNote">
      <skos:prefLabel xml:lang="en">Xl note</skos:prefLabel>
   </rdf:Description>
   <rdf:Description rdf:about="http://publications.europa.eu/ontology/euvoc#XlNote">
      <skos:definition xml:lang="en">Like the skosxl:Label class reifies SKOS label statements, XlNote reifies SKOS note statements (i.e. skos:editorialNote, skos:example, skos:historyNote, skos:definition, skos:scopeNote and skos:changeNote). This class permits, if needed, to maintain the historical view of the values and add additional provenance descriptions.</skos:definition>
   </rdf:Description>
   <owl:Class rdf:about="http://www.w3.org/2004/02/skos/core#Concept"/>
   <rdf:Description rdf:about="http://www.w3.org/2004/02/skos/core#Concept">
      <skos:prefLabel xml:lang="en">Concept</skos:prefLabel>
   </rdf:Description>
   <rdf:Description rdf:about="http://www.w3.org/2004/02/skos/core#Concept">
      <skos:definition xml:lang="en">A concept is a unit of thought. The semantic content of a concept can be re-expressed by a combination of other and different concepts, which may vary from one language or culture to another. Concepts exist in the mind as abstract entities that are independent of the terms used to label them.</skos:definition>
   </rdf:Description>
   <owl:Class rdf:about="http://www.w3.org/2004/02/skos/core#ConceptScheme"/>
   <rdf:Description rdf:about="http://www.w3.org/2004/02/skos/core#ConceptScheme">
      <skos:prefLabel xml:lang="en">Concept scheme</skos:prefLabel>
   </rdf:Description>
   <rdf:Description rdf:about="http://www.w3.org/2004/02/skos/core#ConceptScheme">
      <skos:definition xml:lang="en">A concept schema is a set of concepts, which may include statements about the semantic relationships between those concepts. Thesauri, classification schemes, subject heading lists, taxonomies, terminologies, glossaries, and other types of controlled vocabularies are examples of concept schemas.</skos:definition>
   </rdf:Description>
   <owl:Class rdf:about="http://www.w3.org/2008/05/skos-xl#Label"/>
   <rdf:Description rdf:about="http://www.w3.org/2008/05/skos-xl#Label">
      <skos:prefLabel xml:lang="en">Label</skos:prefLabel>
   </rdf:Description>
   <rdf:Description rdf:about="http://www.w3.org/2008/05/skos-xl#Label">
      <skos:definition xml:lang="en">The class skosxl:Label is a special class of lexical entities. An instance of the class skosxl:Label is a resource and may be named with a URI. An instance of the class skosxl:Label has a single literal form. This literal form is an RDF plain literal (which is a string of UNICODE characters and an optional language tag [&lt;xref scope="external" href="https://www.w3.org/TR/rdf-concepts/"&gt;&lt;foreign otherprops="#0000ff"&gt;&lt;u&gt;RDF-CONCEPTS&lt;/u&gt;&lt;/foreign&gt;&lt;/xref&gt;]). The property skosxl:literalForm is used to give the literal form of an skosxl:Label. If two instances of the class skosxl:Label have the same literal form, they are not necessarily the same resource.</skos:definition>
   </rdf:Description>
   <skos:ConceptScheme rdf:about="http://publications.europa.eu/resource/authority/concept-status"/>
   <rdf:Description rdf:about="http://publications.europa.eu/resource/authority/concept-status">
      <skos:prefLabel xml:lang="en">Concept-status</skos:prefLabel>
   </rdf:Description>
   <rdf:Description rdf:about="http://publications.europa.eu/resource/authority/concept-status">
      <skos:definition xml:lang="en">The Concept status authority table is an internal controlled vocabulary used at the Publications Office. It provides the various statuses used in a harmonised way amongst the authority tables. Concepts with current, deprecated and retired statuses are published while the remaining statuses are related to the internal workflow.</skos:definition>
   </rdf:Description>
   <skos:ConceptScheme rdf:about="http://publications.europa.eu/resource/authority/correction-status"/>
   <rdf:Description rdf:about="http://publications.europa.eu/resource/authority/correction-status">
      <skos:prefLabel xml:lang="en">Correction-status</skos:prefLabel>
   </rdf:Description>
   <skos:ConceptScheme rdf:about="http://publications.europa.eu/resource/authority/gramatical-gender"/>
   <rdf:Description rdf:about="http://publications.europa.eu/resource/authority/gramatical-gender">
      <skos:prefLabel xml:lang="en">Gramatical-gender</skos:prefLabel>
   </rdf:Description>
   <rdf:Description rdf:about="http://publications.europa.eu/resource/authority/gramatical-gender">
      <skos:definition xml:lang="en">The grammatical-gender authority table is a controlled vocabulary which provides the list of the grammatical genders in languages which have gender distinctions: "male", "female", "neuter" or "utrum". It also contains concepts for "no gender" (in languages that do not have gender distinctions) and "generic" (identical forms in languages that make gender distinctions).</skos:definition>
   </rdf:Description>
   <skos:ConceptScheme rdf:about="http://publications.europa.eu/resource/authority/grammatical-number"/>
   <rdf:Description rdf:about="http://publications.europa.eu/resource/authority/grammatical-number">
      <skos:prefLabel xml:lang="en">Grammatical-number</skos:prefLabel>
   </rdf:Description>
   <rdf:Description rdf:about="http://publications.europa.eu/resource/authority/grammatical-number">
      <skos:definition xml:lang="en">The grammatical-number authority table is a controlled vocabulary which provides the list of the grammatical numbers referring to different number of things or persons: "singular", "dual" or "plural". There is also a concept "generic" for forms that do not distinguish between grammatical numbers.</skos:definition>
   </rdf:Description>
   <skos:ConceptScheme rdf:about="http://publications.europa.eu/resource/authority/label-type"/>
   <rdf:Description rdf:about="http://publications.europa.eu/resource/authority/label-type">
      <skos:prefLabel xml:lang="en">Label-type</skos:prefLabel>
   </rdf:Description>
   <rdf:Description rdf:about="http://publications.europa.eu/resource/authority/label-type">
      <skos:definition xml:lang="en">The label-type authority table is a controlled vocabulary providing the various forms of labels that are considered alternative labels in the SKOS format. This authority table is an internal table at the Publications Office of the European Union.</skos:definition>
   </rdf:Description>
   <skos:ConceptScheme rdf:about="http://publications.europa.eu/resource/authority/notation-type"/>
   <rdf:Description rdf:about="http://publications.europa.eu/resource/authority/notation-type">
      <skos:prefLabel xml:lang="en">Notation-type</skos:prefLabel>
   </rdf:Description>
   <rdf:Description rdf:about="http://publications.europa.eu/resource/authority/notation-type">
      <skos:definition xml:lang="en">The Notation type authority table is a controlled vocabulary providing the list of notation types used in the EU Vocabularies authority tables as well as in the context of DCAT-AP (a specification based on W3C's Data Catalogue vocabulary). It indicates the authority code and start-use date of each concept.</skos:definition>
   </rdf:Description>
   <skos:ConceptScheme rdf:about="http://publications.europa.eu/resource/authority/script"/>
   <rdf:Description rdf:about="http://publications.europa.eu/resource/authority/script">
      <skos:prefLabel xml:lang="en">Script</skos:prefLabel>
   </rdf:Description>
   <rdf:Description rdf:about="http://publications.europa.eu/resource/authority/script">
      <skos:definition xml:lang="en">The Script authority table is a controlled vocabulary that lists concepts associated with distinctive scripts. Its main scope is to support activities associated with publication process. The concepts included are correlated with the ISO 15924 international standard. Each script is instantiated according to a writing system, described in writing-system authority table.</skos:definition>
   </rdf:Description>
   <skos:ConceptScheme rdf:about="http://publications.europa.eu/resource/authority/use-context"/>
   <rdf:Description rdf:about="http://publications.europa.eu/resource/authority/use-context">
      <skos:prefLabel xml:lang="en">Use-context</skos:prefLabel>
   </rdf:Description>
   <rdf:Description rdf:about="http://publications.europa.eu/resource/authority/use-context">
      <skos:definition xml:lang="en">The Use context authority table is a controlled vocabulary listing different applications and environments that make use of the various authority tables.</skos:definition>
   </rdf:Description>
   <owl:NamedIndividual rdf:about="http://publications.europa.eu/resource/authority/label-type">
      <rdf:type rdf:resource="http://www.w3.org/2004/02/skos/core#ConceptScheme"/>
   </owl:NamedIndividual>
   <owl:NamedIndividual rdf:about="http://publications.europa.eu/resource/authority/corporate-body">
      <rdf:type rdf:resource="http://www.w3.org/2004/02/skos/core#ConceptScheme"/>
   </owl:NamedIndividual>
   <owl:NamedIndividual rdf:about="http://publications.europa.eu/resource/authority/treaty">
      <rdf:type rdf:resource="http://www.w3.org/2004/02/skos/core#ConceptScheme"/>
   </owl:NamedIndividual>
   <owl:NamedIndividual rdf:about="http://publications.europa.eu/resource/authority/site">
      <rdf:type rdf:resource="http://www.w3.org/2004/02/skos/core#ConceptScheme"/>
   </owl:NamedIndividual>
   <owl:NamedIndividual rdf:about="http://publications.europa.eu/resource/authority/gramatical-gender">
      <rdf:type rdf:resource="http://www.w3.org/2004/02/skos/core#ConceptScheme"/>
   </owl:NamedIndividual>
   <owl:NamedIndividual rdf:about="http://publications.europa.eu/resource/authority/site">
      <rdf:type rdf:resource="http://www.w3.org/2004/02/skos/core#ConceptScheme"/>
   </owl:NamedIndividual>
   <owl:NamedIndividual rdf:about="http://publications.europa.eu/resource/authority/currency">
      <rdf:type rdf:resource="http://www.w3.org/2004/02/skos/core#ConceptScheme"/>
   </owl:NamedIndividual>
   <owl:NamedIndividual rdf:about="http://publications.europa.eu/resource/authority/script">
      <rdf:type rdf:resource="http://www.w3.org/2004/02/skos/core#ConceptScheme"/>
   </owl:NamedIndividual>
   <owl:NamedIndividual rdf:about="http://publications.europa.eu/resource/authority/capital-classification">
      <rdf:type rdf:resource="http://www.w3.org/2004/02/skos/core#ConceptScheme"/>
   </owl:NamedIndividual>
   <owl:NamedIndividual rdf:about="http://publications.europa.eu/resource/authority/correction-status">
      <rdf:type rdf:resource="http://www.w3.org/2004/02/skos/core#ConceptScheme"/>
   </owl:NamedIndividual>
   <owl:NamedIndividual rdf:about="http://publications.europa.eu/resource/authority/language">
      <rdf:type rdf:resource="http://www.w3.org/2004/02/skos/core#ConceptScheme"/>
   </owl:NamedIndividual>
   <owl:NamedIndividual rdf:about="http://publications.europa.eu/resource/authority/concept-status">
      <rdf:type rdf:resource="http://www.w3.org/2004/02/skos/core#ConceptScheme"/>
   </owl:NamedIndividual>
   <owl:NamedIndividual rdf:about="http://publications.europa.eu/resource/authority/grammatical-number">
      <rdf:type rdf:resource="http://www.w3.org/2004/02/skos/core#ConceptScheme"/>
   </owl:NamedIndividual>
   <owl:NamedIndividual rdf:about="http://publications.europa.eu/resource/authority/place">
      <rdf:type rdf:resource="http://www.w3.org/2004/02/skos/core#ConceptScheme"/>
   </owl:NamedIndividual>
   <owl:NamedIndividual rdf:about="http://publications.europa.eu/resource/authority/notation-type">
      <rdf:type rdf:resource="http://www.w3.org/2004/02/skos/core#ConceptScheme"/>
   </owl:NamedIndividual>
   <owl:NamedIndividual rdf:about="http://publications.europa.eu/resource/authority/country">
      <rdf:type rdf:resource="http://www.w3.org/2004/02/skos/core#ConceptScheme"/>
   </owl:NamedIndividual>
   <owl:NamedIndividual rdf:about="http://publications.europa.eu/resource/authority/use-context">
      <rdf:type rdf:resource="http://www.w3.org/2004/02/skos/core#ConceptScheme"/>
   </owl:NamedIndividual>
   <owl:Class rdf:about="http://publications.europa.eu/ontology/euvoc#ConceptStatus">
      <rdfs:subClassOf rdf:resource="http://www.w3.org/2004/02/skos/core#Concept"/>
   </owl:Class>
   <owl:Class rdf:about="http://publications.europa.eu/ontology/euvoc#CorrectionStatus">
      <rdfs:subClassOf rdf:resource="http://www.w3.org/2004/02/skos/core#Concept"/>
   </owl:Class>
   <owl:Class rdf:about="http://publications.europa.eu/ontology/euvoc#GrammaticalGender">
      <rdfs:subClassOf rdf:resource="http://www.w3.org/2004/02/skos/core#Concept"/>
   </owl:Class>
   <owl:Class rdf:about="http://publications.europa.eu/ontology/euvoc#LabelType">
      <rdfs:subClassOf rdf:resource="http://www.w3.org/2004/02/skos/core#Concept"/>
   </owl:Class>
   <owl:Class rdf:about="http://publications.europa.eu/ontology/euvoc#NotationType">
      <rdfs:subClassOf rdf:resource="http://www.w3.org/2004/02/skos/core#Concept"/>
   </owl:Class>
   <owl:Class rdf:about="http://publications.europa.eu/ontology/euvoc#Script">
      <rdfs:subClassOf rdf:resource="http://www.w3.org/2004/02/skos/core#Concept"/>
   </owl:Class>
   <owl:Class rdf:about="http://publications.europa.eu/ontology/euvoc#UseContext">
      <rdfs:subClassOf rdf:resource="http://www.w3.org/2004/02/skos/core#Concept"/>
   </owl:Class>
   <owl:ObjectProperty rdf:about="http://www.w3.org/2004/02/skos/core#inScheme"/>
   <rdf:Description rdf:about="http://www.w3.org/2004/02/skos/core#inScheme">
      <skos:prefLabel xml:lang="en">In scheme</skos:prefLabel>
   </rdf:Description>
   <rdf:Description rdf:about="http://www.w3.org/2004/02/skos/core#inScheme">
      <skos:definition xml:lang="en">A Concept Scheme in which the Concept is included. A Concept may be a member of more than one concept scheme. (skos:Concept -&gt; skos:ConceptScheme (+skos:inScheme))</skos:definition>
   </rdf:Description>
   <owl:ObjectProperty rdf:about="http://purl.org/dc/terms/type"/>
   <rdf:Description rdf:about="http://purl.org/dc/terms/type">
      <skos:prefLabel xml:lang="en">Type</skos:prefLabel>
   </rdf:Description>
   <rdf:Description rdf:about="http://purl.org/dc/terms/type">
      <skos:definition xml:lang="en">Specify the context where a specified notation is considered unique. (euvoc:XlNotation -&gt; at-voc:notation-type (+dct:type))</skos:definition>
   </rdf:Description>
   <owl:ObjectProperty rdf:about="http://publications.europa.eu/ontology/euvoc#xlNotation"/>
   <rdf:Description rdf:about="http://publications.europa.eu/ontology/euvoc#xlNotation">
      <skos:prefLabel xml:lang="en">Xl notation</skos:prefLabel>
   </rdf:Description>
   <rdf:Description rdf:about="http://publications.europa.eu/ontology/euvoc#xlNotation">
      <skos:definition xml:lang="en">A notation is a string of characters such as "T58.5" or "303.4833" used to uniquely identify a concept within the scope of a given concept scheme or within a specified context. (skos:Concept -&gt; euvoc:XlNotation (+euvoc:xlNotation))</skos:definition>
   </rdf:Description>
   <owl:ObjectProperty rdf:about="http://publications.europa.eu/ontology/euvoc#corrStatus"/>
   <rdf:Description rdf:about="http://publications.europa.eu/ontology/euvoc#corrStatus">
      <skos:prefLabel xml:lang="en">Corr status</skos:prefLabel>
   </rdf:Description>
   <rdf:Description rdf:about="http://publications.europa.eu/ontology/euvoc#corrStatus">
      <skos:definition xml:lang="en">A status of proofreading of labels and descriptions. (euvoc:XlNote -&gt; at-voc:correction-status (+euvoc:corrStatus)) A status of proofreading of labels and descriptions. (skosxl:Label -&gt; at-voc:correction-status (+euvoc:corrStatus))</skos:definition>
   </rdf:Description>
   <owl:ObjectProperty rdf:about="http://publications.europa.eu/ontology/euvoc#xlHistoryNote"/>
   <rdf:Description rdf:about="http://publications.europa.eu/ontology/euvoc#xlHistoryNote">
      <skos:prefLabel xml:lang="en">Xl history note</skos:prefLabel>
   </rdf:Description>
   <rdf:Description rdf:about="http://publications.europa.eu/ontology/euvoc#xlHistoryNote">
      <skos:definition xml:lang="en">A note about the past state/use/meaning of a concept. (skos:Concept -&gt; euvoc:XlNote (+euvoc:xlHistoryNote))</skos:definition>
   </rdf:Description>
   <owl:ObjectProperty rdf:about="http://publications.europa.eu/ontology/euvoc#xlNote"/>
   <rdf:Description rdf:about="http://publications.europa.eu/ontology/euvoc#xlNote">
      <skos:prefLabel xml:lang="en">Xl note</skos:prefLabel>
   </rdf:Description>
   <owl:ObjectProperty rdf:about="http://publications.europa.eu/ontology/euvoc#xlChangeNote"/>
   <rdf:Description rdf:about="http://publications.europa.eu/ontology/euvoc#xlChangeNote">
      <skos:prefLabel xml:lang="en">Xl change note</skos:prefLabel>
   </rdf:Description>
   <rdf:Description rdf:about="http://publications.europa.eu/ontology/euvoc#xlChangeNote">
      <skos:definition xml:lang="en">A note about a modification to a concept. (skos:Concept -&gt; euvoc:XlNote (+euvoc:xlChangeNote))</skos:definition>
   </rdf:Description>
   <owl:ObjectProperty rdf:about="http://publications.europa.eu/ontology/euvoc#xlDefinition"/>
   <rdf:Description rdf:about="http://publications.europa.eu/ontology/euvoc#xlDefinition">
      <skos:prefLabel xml:lang="en">Xl definition</skos:prefLabel>
   </rdf:Description>
   <rdf:Description rdf:about="http://publications.europa.eu/ontology/euvoc#xlDefinition">
      <skos:definition xml:lang="en">A statement or formal explanation of the meaning of a concept. (skos:Concept -&gt; euvoc:XlNote (+euvoc:xlDefinition))</skos:definition>
   </rdf:Description>
   <owl:ObjectProperty rdf:about="http://www.w3.org/2008/05/skos-xl#altLabel"/>
   <rdf:Description rdf:about="http://www.w3.org/2008/05/skos-xl#altLabel">
      <skos:prefLabel xml:lang="en">Alt label</skos:prefLabel>
   </rdf:Description>
   <rdf:Description rdf:about="http://www.w3.org/2008/05/skos-xl#altLabel">
      <skos:definition xml:lang="en">An alternative lexical label for a resource. Acronyms, abbreviations, spelling variants, and irregular plural/singular forms may be included among the alternative labels for a concept. (skos:Concept -&gt; skosxl:Label (+skosxl:altLabel))</skos:definition>
   </rdf:Description>
   <owl:ObjectProperty rdf:about="http://www.w3.org/2008/05/skos-xl#prefLabel"/>
   <rdf:Description rdf:about="http://www.w3.org/2008/05/skos-xl#prefLabel">
      <skos:prefLabel xml:lang="en">Pref label</skos:prefLabel>
   </rdf:Description>
   <rdf:Description rdf:about="http://www.w3.org/2008/05/skos-xl#prefLabel">
      <skos:definition xml:lang="en">The preferred lexical label for a resource, in a given language. No two concepts in the same concept scheme may have the same preferred label in a given language. (skos:Concept -&gt; skosxl:Label (+skosxl:prefLabel))</skos:definition>
   </rdf:Description>
   <owl:ObjectProperty rdf:about="http://www.w3.org/2004/02/skos/core#exactMatch"/>
   <rdf:Description rdf:about="http://www.w3.org/2004/02/skos/core#exactMatch">
      <skos:prefLabel xml:lang="en">Exact match</skos:prefLabel>
   </rdf:Description>
   <rdf:Description rdf:about="http://www.w3.org/2004/02/skos/core#exactMatch">
      <skos:definition xml:lang="en">The property skos:exactMatch is used to link two concepts, indicating a high degree of confidence that the concepts can be used interchangeably across a wide range of information retrieval applications. skos:exactMatch is a transitive property, and is a sub-property of skos:closeMatch. (skos:Concept -&gt; skos:Concept (+skos:exactMatch))</skos:definition>
   </rdf:Description>
   <owl:ObjectProperty rdf:about="http://www.w3.org/2004/02/skos/core#topConceptOf"/>
   <rdf:Description rdf:about="http://www.w3.org/2004/02/skos/core#topConceptOf">
      <skos:prefLabel xml:lang="en">Top concept of</skos:prefLabel>
   </rdf:Description>
   <rdf:Description rdf:about="http://www.w3.org/2004/02/skos/core#topConceptOf">
      <skos:definition xml:lang="en">A concept scheme in which the concept is included. A concept may be a member of more than one concept scheme. (skos:Concept -&gt; skos:ConceptScheme (+skos:topConceptOf))</skos:definition>
   </rdf:Description>
   <owl:ObjectProperty rdf:about="http://purl.org/dc/terms/isReplacedBy"/>
   <rdf:Description rdf:about="http://purl.org/dc/terms/isReplacedBy">
      <skos:prefLabel xml:lang="en">Is replaced by</skos:prefLabel>
   </rdf:Description>
   <rdf:Description rdf:about="http://purl.org/dc/terms/isReplacedBy">
      <skos:definition xml:lang="en">A related resource that supplants, displaces, or supersedes the described resource. (skos:Concept -&gt; skos:Concept (+dct:isReplacedBy))</skos:definition>
   </rdf:Description>
   <owl:ObjectProperty rdf:about="http://www.w3.org/2004/02/skos/core#narrower"/>
   <rdf:Description rdf:about="http://www.w3.org/2004/02/skos/core#narrower">
      <skos:prefLabel xml:lang="en">Narrower</skos:prefLabel>
   </rdf:Description>
   <rdf:Description rdf:about="http://www.w3.org/2004/02/skos/core#narrower">
      <skos:definition xml:lang="en">A concept that is less general in meaning. Narrower concepts are typically rendered as children in a concept hierarchy (tree). (skos:Concept -&gt; skos:Concept (+skos:narrower))</skos:definition>
   </rdf:Description>
   <owl:ObjectProperty rdf:about="http://www.w3.org/2004/02/skos/core#broader"/>
   <rdf:Description rdf:about="http://www.w3.org/2004/02/skos/core#broader">
      <skos:prefLabel xml:lang="en">Broader</skos:prefLabel>
   </rdf:Description>
   <rdf:Description rdf:about="http://www.w3.org/2004/02/skos/core#broader">
      <skos:definition xml:lang="en">A concept that is more general in meaning. Broader concepts are typically rendered as parents in a concept hierarchy (tree). (skos:Concept -&gt; skos:Concept (+skos:broader))</skos:definition>
   </rdf:Description>
   <owl:ObjectProperty rdf:about="http://publications.europa.eu/ontology/euvoc#context"/>
   <rdf:Description rdf:about="http://publications.europa.eu/ontology/euvoc#context">
      <skos:prefLabel xml:lang="en">Context</skos:prefLabel>
   </rdf:Description>
   <rdf:Description rdf:about="http://publications.europa.eu/ontology/euvoc#context">
      <skos:definition xml:lang="en">It signifies that the concept is applicable or relevant within the context of the identified use context. (skos:Concept -&gt; at-voc:use-context (+euvoc:context))</skos:definition>
   </rdf:Description>
   <owl:ObjectProperty rdf:about="http://www.w3.org/2008/05/skos-xl#hiddenLabel"/>
   <rdf:Description rdf:about="http://www.w3.org/2008/05/skos-xl#hiddenLabel">
      <skos:prefLabel xml:lang="en">Hidden label</skos:prefLabel>
   </rdf:Description>
   <rdf:Description rdf:about="http://www.w3.org/2008/05/skos-xl#hiddenLabel">
      <skos:definition xml:lang="en">A lexical label for a resource that should be hidden when generating visual displays of the resource, but should still be accessible to free text search operations. Mis-spelled terms are normally included as hidden labels. (skos:Concept -&gt; skosxl:Label (+skosxl:hiddenLabel))</skos:definition>
   </rdf:Description>
   <owl:ObjectProperty rdf:about="http://purl.org/dc/terms/replaces"/>
   <rdf:Description rdf:about="http://purl.org/dc/terms/replaces">
      <skos:prefLabel xml:lang="en">Replaces</skos:prefLabel>
   </rdf:Description>
   <rdf:Description rdf:about="http://purl.org/dc/terms/replaces">
      <skos:definition xml:lang="en">A related resource that is supplanted, displaced, or superseded by the described resource. (skos:Concept -&gt; skos:Concept (+dct:replaces))</skos:definition>
   </rdf:Description>
   <owl:ObjectProperty rdf:about="http://publications.europa.eu/ontology/euvoc#status"/>
   <rdf:Description rdf:about="http://publications.europa.eu/ontology/euvoc#status">
      <skos:prefLabel xml:lang="en">Status</skos:prefLabel>
   </rdf:Description>
   <owl:ObjectProperty rdf:about="http://www.w3.org/2004/02/skos/core#hasTopConcept"/>
   <rdf:Description rdf:about="http://www.w3.org/2004/02/skos/core#hasTopConcept">
      <skos:prefLabel xml:lang="en">Has top concept</skos:prefLabel>
   </rdf:Description>
   <owl:ObjectProperty rdf:about="http://www.lexinfo.net/ontology/2.0/lexinfo#gender"/>
   <rdf:Description rdf:about="http://www.lexinfo.net/ontology/2.0/lexinfo#gender">
      <skos:prefLabel xml:lang="en">Gender</skos:prefLabel>
   </rdf:Description>
   <rdf:Description rdf:about="http://www.lexinfo.net/ontology/2.0/lexinfo#gender">
      <skos:definition xml:lang="en">A grammatical category that indicates grammatical relationships between words in sentences. (skosxl:Label -&gt; at-voc:gramatical-gender (+lexinfo:gender))</skos:definition>
   </rdf:Description>
   <owl:ObjectProperty rdf:about="http://lexvo.org/ontology#inScript"/>
   <rdf:Description rdf:about="http://lexvo.org/ontology#inScript">
      <skos:prefLabel xml:lang="en">In script</skos:prefLabel>
   </rdf:Description>
   <owl:ObjectProperty rdf:about="http://www.lexinfo.net/ontology/2.0/lexinfo#number"/>
   <rdf:Description rdf:about="http://www.lexinfo.net/ontology/2.0/lexinfo#number">
      <skos:prefLabel xml:lang="en">Number</skos:prefLabel>
   </rdf:Description>
   <rdf:Description rdf:about="http://www.lexinfo.net/ontology/2.0/lexinfo#number">
      <skos:definition xml:lang="en">Grammatical category for the variation in form of nouns, pronouns, and any words agreeing with them, depending on how many persons or things are referred to. (skosxl:Label -&gt; at-voc:grammatical-number (+lexinfo:number))</skos:definition>
   </rdf:Description>
   <owl:DatatypeProperty rdf:about="http://purl.org/dc/terms/created"/>
   <rdf:Description rdf:about="http://purl.org/dc/terms/created">
      <skos:prefLabel xml:lang="en">Created</skos:prefLabel>
   </rdf:Description>
   <rdf:Description rdf:about="http://purl.org/dc/terms/created">
      <skos:definition xml:lang="en">Date of creation of the resource. (euvoc:XlNotation) Date of creation of the resource. (euvoc:XlNote) Date of creation of the resource. (skos:Concept) Date of creation of the resource. (skos:ConceptScheme) Date of creation of the resource. (skosxl:Label)</skos:definition>
   </rdf:Description>
   <owl:DatatypeProperty rdf:about="http://purl.org/dc/terms/modified"/>
   <rdf:Description rdf:about="http://purl.org/dc/terms/modified">
      <skos:prefLabel xml:lang="en">Modified</skos:prefLabel>
   </rdf:Description>
   <rdf:Description rdf:about="http://purl.org/dc/terms/modified">
      <skos:definition xml:lang="en">Date of modification of the resource. (euvoc:XlNotation) Date of modification of the resource. (euvoc:XlNote) Date of modification of the resource. (skos:Concept) Date of modification of the resource. (skos:ConceptScheme) Date of modification of the resource. (skosxl:Label)</skos:definition>
   </rdf:Description>
   <owl:DatatypeProperty rdf:about="http://publications.europa.eu/ontology/euvoc#endDate"/>
   <rdf:Description rdf:about="http://publications.europa.eu/ontology/euvoc#endDate">
      <skos:prefLabel xml:lang="en">End date</skos:prefLabel>
   </rdf:Description>
   <rdf:Description rdf:about="http://publications.europa.eu/ontology/euvoc#endDate">
      <skos:definition xml:lang="en">End of the validity period. If a resource has an end date then it must be marked as deprecated. (euvoc:XlNotation) End of the validity period. If a resource has an end date then it must be marked as deprecated. (euvoc:XlNote) End of the validity period. If a resource has an end date then it must be marked as deprecated. (skos:Concept) End of the validity period. If a resource has an end date then it must be marked as deprecated. (skos:ConceptScheme) End of the validity period. If a resource has an end date then it must be marked as deprecated. (skosxl:Label)</skos:definition>
   </rdf:Description>
   <owl:DatatypeProperty rdf:about="http://publications.europa.eu/ontology/euvoc#startDate"/>
   <rdf:Description rdf:about="http://publications.europa.eu/ontology/euvoc#startDate">
      <skos:prefLabel xml:lang="en">Start date</skos:prefLabel>
   </rdf:Description>
   <rdf:Description rdf:about="http://publications.europa.eu/ontology/euvoc#startDate">
      <skos:definition xml:lang="en">Beginning of the validity period. (euvoc:XlNotation) Beginning of the validity period. (euvoc:XlNote) Beginning of the validity period. (skos:Concept) Beginning of the validity period. (skos:ConceptScheme) Beginning of the validity period. (skosxl:Label)</skos:definition>
   </rdf:Description>
   <owl:DatatypeProperty rdf:about="http://www.w3.org/2002/07/owl#deprecated"/>
   <rdf:Description rdf:about="http://www.w3.org/2002/07/owl#deprecated">
      <skos:prefLabel xml:lang="en">Deprecated</skos:prefLabel>
   </rdf:Description>
   <rdf:Description rdf:about="http://www.w3.org/2002/07/owl#deprecated">
      <skos:definition xml:lang="en">States whether the resource is current or deprecated. By deprecating a resource, it means that it should not be used in new documents. Deprecation is a feature commonly used in versioning software to indicate that a particular feature is preserved for backward-compatibility purposes, but may be phased out in the future. (euvoc:XlNotation) States whether the resource is current or deprecated. By deprecating a resource, it means that it should not be used in new documents. Deprecation is a feature commonly used in versioning software to indicate that a particular feature is preserved for backward-compatibility purposes, but may be phased out in the future. (euvoc:XlNote) States whether the resource is current or deprecated. By deprecating a resource, it means that it should not be used in new documents. Deprecation is a feature commonly used in versioning software to indicate that a particular feature is preserved for backward-compatibility purposes, but may be phased out in the future (skos:Concept) States whether the resource is current or deprecated. By deprecating a resource, it means that it should not be used in new documents. Deprecation is a feature commonly used in versioning software to indicate that a particular feature is preserved for backward-compatibility purposes, but may be phased out in the future (skos:ConceptScheme) States whether the resource is current or deprecated. By deprecating a resource, it means that it should not be used in new documents. Deprecation is a feature commonly used in versioning software to indicate that a particular feature is preserved for backward-compatibility purposes, but may be phased out in the future. (skosxl:Label)</skos:definition>
   </rdf:Description>
   <owl:DatatypeProperty rdf:about="http://www.w3.org/1999/02/22-rdf-syntax-ns#value"/>
   <rdf:Description rdf:about="http://www.w3.org/1999/02/22-rdf-syntax-ns#value">
      <skos:prefLabel xml:lang="en">Value</skos:prefLabel>
   </rdf:Description>
   <rdf:Description rdf:about="http://www.w3.org/1999/02/22-rdf-syntax-ns#value">
      <skos:definition xml:lang="en">The literal form of the note. (euvoc:XlNotation) The literal form of the note. (euvoc:XlNote)</skos:definition>
   </rdf:Description>
   <owl:DatatypeProperty rdf:about="http://purl.org/dc/terms/creator"/>
   <rdf:Description rdf:about="http://purl.org/dc/terms/creator">
      <skos:prefLabel xml:lang="en">Creator</skos:prefLabel>
   </rdf:Description>
   <rdf:Description rdf:about="http://purl.org/dc/terms/creator">
      <skos:definition xml:lang="en">The entity or entities responsible for creating the resource, (euvoc:XlNote)</skos:definition>
   </rdf:Description>
   <owl:DatatypeProperty rdf:about="http://purl.org/dc/terms/dateAccepted"/>
   <rdf:Description rdf:about="http://purl.org/dc/terms/dateAccepted">
      <skos:prefLabel xml:lang="en">Date accepted</skos:prefLabel>
   </rdf:Description>
   <rdf:Description rdf:about="http://purl.org/dc/terms/dateAccepted">
      <skos:definition xml:lang="en">Date of acceptance of the resource. (skos:Concept)</skos:definition>
   </rdf:Description>
   <owl:DatatypeProperty rdf:about="http://purl.org/dc/terms/dateSubmitted"/>
   <rdf:Description rdf:about="http://purl.org/dc/terms/dateSubmitted">
      <skos:prefLabel xml:lang="en">Date submitted</skos:prefLabel>
   </rdf:Description>
   <rdf:Description rdf:about="http://purl.org/dc/terms/dateSubmitted">
      <skos:definition xml:lang="en">Date of submission of the resource. (skos:Concept)</skos:definition>
   </rdf:Description>
   <rdf:Property rdf:about="http://www.w3.org/2002/07/owl#versionInfo"/>
   <rdf:Description rdf:about="http://www.w3.org/2002/07/owl#versionInfo">
      <skos:prefLabel xml:lang="en">Version info</skos:prefLabel>
   </rdf:Description>
   <rdf:Description rdf:about="http://www.w3.org/2002/07/owl#versionInfo">
      <skos:definition xml:lang="en">An owl:versionInfo statement generally has as its object a string giving information about this version. This statement does not contribute to the logical meaning of the resource. (skos:Concept) An owl:versionInfo statement generally has as its object a string giving information about this version. This statement does not contribute to the logical meaning of the resource. (skos:ConceptScheme)</skos:definition>
   </rdf:Description>
   <owl:DatatypeProperty rdf:about="http://purl.org/dc/terms/identifier"/>
   <rdf:Description rdf:about="http://purl.org/dc/terms/identifier">
      <skos:prefLabel xml:lang="en">Identifier</skos:prefLabel>
   </rdf:Description>
   <rdf:Description rdf:about="http://purl.org/dc/terms/identifier">
      <skos:definition xml:lang="en">An unambiguous reference to the resource within a given context. Recommended best practice is to identify the resource by means of a string conforming to a formal identification system. (skos:ConceptScheme)</skos:definition>
   </rdf:Description>
   <owl:DatatypeProperty rdf:about="http://purl.org/dc/terms/title"/>
   <rdf:Description rdf:about="http://purl.org/dc/terms/title">
      <skos:prefLabel xml:lang="en">Title</skos:prefLabel>
   </rdf:Description>
   <rdf:Description rdf:about="http://purl.org/dc/terms/title">
      <skos:definition xml:lang="en">It represents the title or name of a resource. (skos:ConceptScheme)</skos:definition>
   </rdf:Description>
   <owl:DatatypeProperty rdf:about="http://www.w3.org/2008/05/skos-xl#literalForm"/>
   <rdf:Description rdf:about="http://www.w3.org/2008/05/skos-xl#literalForm">
      <skos:prefLabel xml:lang="en">Literal form</skos:prefLabel>
   </rdf:Description>
   <rdf:Description rdf:about="http://www.w3.org/2008/05/skos-xl#literalForm">
      <skos:definition xml:lang="en">An instance of the class skosxl:Label has one and only one literal form. (skosxl:Label)</skos:definition>
   </rdf:Description>
</rdf:RDF>
